\begin{tabular}{| l | l |}
    \hline
    \begin{tabular}{l}
        Volume of a cylinder: $V=h \pi r^2$
    \end{tabular}
    &
    \begin{tabular}{l}
        Surface area of a cylinder: $A=(2 \pi r^2) + (2 \pi r h)$
    \end{tabular} \\
    \hline
\end{tabular}

\begin{tabular}{| l | l | l | l |}
    \hline
    \begin{tabular}{l}
        \textbf{1. Isolate h} \\
        \textbf{for surface area.} \\
        $A=(2 \pi r^2) + (2 \pi r h)$ \\\\
        $2 \pi r^2 = A - 2 \pi r^2$ \\\\
        $h = \frac{A - 2 \pi r^2}{2 \pi r}$ \\\\\\\\\\\\\\\\
    \end{tabular}
&
    \begin{tabular}{l}
        \textbf{2. Insert the} \\
        \textbf{volume formula.} \\
        $h = \frac{A - 2 \pi r^2}{2 pi r}$ \\\\
        $V=h \pi r^2$ \\\\
        $V= (\frac{A - 2 \pi r^2}{2 \pi r}) \pi r^2$ \\\\
        $V = \frac{(A \pi r^2) - (2 \pi^2 r^4)}{2 \pi r}$ \\\\
        $V = \frac{A \pi r^2}{2 \pi r} - \frac{2 \pi^2 r^4}{2 \pi r}$ \\\\
        $V = \frac{A r}{2} - \pi r^3$ \\\\
    \end{tabular}
&
    \begin{tabular}{l}
        \textbf{3. Find derivative.}\\
        $V(r) = \frac{A r}{2} - \pi r^3$ \\\\
        $V'(r) = \frac{A r}{2} - 3 \pi r^2$ \\\\
        $V'(r) = \frac{A}{2} - 3 \pi r^2$ \\\\\\\\\\\\\\\
    \end{tabular}
&
    \begin{tabular}{l}
        \textbf{4. Critical point.}\\
        $V'(r) = \frac{A}{2} - 3 \pi r^2 = 0$ \\\\
        $3 \pi r^2 = \frac{A}{2}$ \\\\
        $r^2 = \frac{A}{(3 \times 2) \pi}$ \\\\
        $r = \sqrt{\frac{A}{(3 \times 2) \pi}}$ \\\\
        $r = \sqrt{\frac{A}{6 \pi}}$ \\\\\
    \end{tabular}
    \\
\hline
\end{tabular}

\begin{tabular}{| l  l | l |}
    \hline
    \textbf{5. Find h for volume} && \textbf{6. Volume} \\
    \begin{tabular}{l}
        $r = \sqrt{\frac{A}{6 \pi}}$ \\\\\
        $h = \frac{A - 2 \pi r^2}{2 \pi r}$ \\\\
        $h = \frac{A - 2 \pi (\sqrt{\frac{A}{6 \pi}})^2}{2 \pi (\sqrt{\frac{A}{6 \pi})}}$ \\\\
        $h = \frac{A - 2 \pi (\frac{A}{6 \pi})}{2 \pi (\sqrt{\frac{A}{6 \pi})}}$ \\\\
        $h = \frac{A - \frac{2 \pi A}{6 \pi}}{2 \pi \sqrt{\frac{ A}{6 \pi}}}$ \\\\
        $h = \frac{A - \frac{A}{3}}{2 \pi \sqrt{\frac{A}{6 \pi}}}$ \\\\
        $h = \frac{\frac{3A}{3} - \frac{A}{3}}{2 \pi \sqrt{\frac{A}{6 \pi}}}$ \\\\
        $h = \frac{\frac{3A - A}{3}}{2 \pi \sqrt{\frac{A}{6 \pi}}}$ \\\\
    \end{tabular}{}
    &
    \begin{tabular}{l}
        %$h = \frac{\frac{2A}{3}}{2 \pi \sqrt{\frac{A}{6 \pi}}}$ \\\\
        
        $h = \frac{\frac{2A}{3}}{2 \pi \sqrt{\frac{A}{6 \pi}}}$ \\\\
        $h = \frac{2A}{3} \times \frac{1}{\sqrt{\frac{2 \pi A}{6 \pi}}}$ \\\\
        $h = \frac{2A}{3} \times \frac{\sqrt{6 \pi}}{2 \pi \sqrt{A}}$ \\\\
        $h = \frac{\sqrt{6 \pi A}}{3 \pi}$\\\\\\\\\\\\\\\\\\\\\\\\\\\
    \end{tabular}{}
    &
    \begin{tabular}{l}
        $V = h \times \pi \times r^2$\\
        $V = \frac{\sqrt{6 \pi A}}{3 \pi} \times \pi \times (\sqrt{\frac{A}{6 \pi}})^2$\\\\
        $V = \frac{\sqrt{6 \pi A}}{3 \pi} \times \pi \times \frac{A}{6 \pi}$\\\\
        $V = \frac{\sqrt{6 \pi A} \times \pi \times A}{3\pi \times \sqrt{A} \times 6\pi}$ \\\\
        $V = \frac{\sqrt{6 \pi A} \times A}{3 \times 6 \pi}$ \\\\
        $\boxed{V = \frac{A \sqrt{6 \pi A}}{18 \pi}}$ \\\\\\\\\\\\\\\\\\\\\\
    \end{tabular}{}
    \\
\hline
\end{tabular}
