\section*{1.}

$f(x) = arctan(x) + ax$

$f'(x) = \frac{1}{x^2 + 1} + a$

$f''(x) = -\frac{2x}{(x^2 + 1)^2}$ \newline

$\frac{1}{x^2 + 1} + a = 0$

$\frac{1}{x^2 + 1} = -a$

$1 = -a(x^2 + 1)$

$1 = -ax^2 - a$

$1 + ax^2 = -a$

$ax^2 = -a - 1$

$x^2 = \frac{-a - 1}{a}$

$x = \pm \sqrt{\frac{-a - 1}{a}}$

$f''(-1.5) = -\frac{2 \times (-1.5)}{((-1.5)^2 + 1)^2} = \frac{-3}{(2.25 + 1)^2} = -\frac{3}{10.5625}$

$f''(-1) = -\frac{2 \times (-1)}{((-1)^2 + 1)^2} = \frac{-2}{(1 + 1)^2} = -\frac{2}{4}$

$f''(-0.5) = -\frac{2 \times (-0.5)}{((-0.5)^2 + 1)^2} = \frac{-1}{(0.25 + 1)^2} = -\frac{1}{1.5625}$

$f''(0) = -\frac{2 \times (0)}{((0)^2 + 1)^2} = \frac{-0}{(0 + 1)^2} = 0$

\begin{tabular}{| l | l | l |}
    \hline
    & & \\
    $- \sqrt{\frac{-a - 1}{a}}$ & Local Minimum & $-1 < a < 0$ \\
    & & \\
    \hline
\end{tabular}

\section*{2.}

$x = -\sqrt{\frac{-a - 1}{a}}$

$x = arctan(-\sqrt{\frac{-a - 1}{a}}) + a(-\sqrt{\frac{-a - 1}{a}}) = -arctan(\sqrt{\frac{-a - 1}{a}}) - a(\sqrt{\frac{-a - 1}{a}})$

$\boxed{(-\sqrt{\frac{-a - 1}{a}}, (-arctan(\sqrt{\frac{-a - 1}{a}}) - a(\sqrt{\frac{-a - 1}{a}})))}$
