\section*{1.}

\subsection*{Order Zero:}

$f(0) = \sqrt{\frac{1}{3+e^0}} = \sqrt{\frac{1}{3+1}} = \sqrt{\frac{1}{4}} = \frac{1}{2}$

\subsection*{Order One:}

$f(x) = \sqrt{\frac{1}{3+e^x}} = (\frac{1}{3 + e^x})^{\frac{1}{2}} =  ((3+e^x)^{-1})^{\frac{1}{2}} $

$f'(x) = -\frac{1}{2}((3+e^x)^{-1})^{\frac{1}{2}} \times e^x = -\frac{1}{2}(3+e^x)^{\frac{3}{2}} \times e^x = - \frac{1}{2(3 + e^x)^{\frac{3}{2}}} \times e^x= - \frac{e^x}{2(3 + e^x)^{\frac{3}{2}}}$

$f'(0) = -\frac{e^0}{2(3+e^0)^{\frac{3}{2}}} = -\frac{1}{2(3+1)^{\frac{3}{2}}} = -\frac{1}{2(4)^\frac{3}{2}} = -\frac{1}{8^{\frac{3}{2}}} = -\frac{1}{16}$

\subsection*{Order Two:}

$f'(x) = -\frac{1}{2}e^x(3 + e^x)^{-\frac{3}{2}} = -\frac{1}{2}(g(x)h(x))$

$g(x) = (3 + e^x)^{-\frac{3}{2}}$

$g'(x) = -\frac{3}{2}(3 + e^x)^{-\frac{5}{2}}$

$h(x) = e^x$

$h'(x) = e^x$

$f''(x) = -\frac{1}{2}(g(x)h'(x) + g'(x)h'(x)) = -\frac{1}{2}(((e^x)((3 + e^x)^{-\frac{3}{2}})+(e^x)((-\frac{3}{2} + e^x)^{-\frac{5}{2}})(e^x)))$

$f''(x) =  \frac{-3e^x + \frac{1}{2}e^{2x}}{2(3+e^x)^{\frac{5}{2}}}$

$f''(0) =  \frac{-3e^0 + \frac{1}{2}e^{2 \times 0}}{2(3+e^0)^{\frac{5}{2}}} = \frac{-3 \times 1 + \frac{1}{2}e^0}{2(3+1)^{\frac{5}{2}}} = \frac{-3 + \frac{1}{2}}{2(3+1)^{\frac{5}{2}}} = \frac{-\frac{5}{2}}{8^{\frac{5}{2}}} = \frac{-\frac{5}{2}}{64} = -\frac{5}{128}$

$f(0) + f'(0)x + f''(0)x^2 = \frac{1}{2} + (\frac{-\frac{1}{16}}{1})x + (\frac{-\frac{5}{128}}{2})x^2 = \boxed{\frac{1}{2} - \frac{1}{16}x - \frac{5}{256}x^2}$

\section*{2.}

\begin{tabular}{l l l}
$\frac{1}{2} - (\frac{1}{16})(0.3) - (\frac{5}{128})(0.3)^2 = \frac{1}{2} - \frac{1}{16}(0.3) - \frac{5}{256}(0.3)^2$ & = & $\boxed{0.4794921875}$ \\\\
$\sqrt{\frac{1}{3+e^{(0.3)}}}$ & = & $\boxed{0.47947108289}$ \\\\
& & \boxed{\text{Four decimal digits match}}. \\
\end{tabular}